thread locks

steel/Zeta.Steel.SafeMain.fst
@@ -5,6 +5,36 @@ module R = Steel.ST.Reference
 
 open Steel.ST.GenElim
 
+// TODO: use FStarLang/FStar#2349 to nest structs and take pointers to fields. However, we need support for atomic accesses for such references, at least for the top-level cases (so far we don't need atomic field accesses here yet)
+
+[@@__reduce__]
+let thread_lock_vprop
+  (tl_state: M.top_level_state)
+  (tid: AT.tid)
+: Tot vprop
+= exists_ (fun (entries: AEH.log) -> M.log_of_tid tl_state tid entries)
+
+let thread_lock_t
+  (tl_state: M.top_level_state)
+: Tot Type
+= (tid: Ghost.erased AT.tid & Lock.lock (thread_lock_vprop tl_state tid))
+
+let thread_state_prop
+  (#tl_state: M.top_level_state)
+  (a: Seq.seq (thread_lock_t tl_state))
+: Tot prop
+= forall (i: nat { i < Seq.length a }) . {:pattern (Seq.index a i)} U16.v (dfst (Seq.index a i)) == i
+
+noeq
+type state_t = {
+  state: R.ref M.top_level_state;
+  tl_state: Ghost.erased M.top_level_state;
+  thread_locks: A.array (thread_lock_t tl_state);
+  tl_thread_locks: Ghost.erased (Seq.seq (thread_lock_t tl_state));
+  tl_frozen_logs: Ghost.erased M.tid_log_map;
+  tl_prf: squash (thread_state_prop tl_thread_locks /\ Seq.length tl_thread_locks == U32.v AT.n_threads);
+}
+
 [@@__reduce__]
 let state_ptr_inv_null
   (p: perm)
@@ -12,13 +42,41 @@ let state_ptr_inv_null
 = pure (p == full_perm)
 
 [@@__reduce__]
-let state_ptr_inv_not_null
-  (state: R.ref M.top_level_state)
+let handle_pts_to_body0
+  (r2: state_t)
 : Tot vprop
-= exists_ (fun pt -> exists_ (fun t -> R.pts_to state pt t `star` M.core_inv t))
+= exists_ (fun p3 -> exists_ (fun p4 ->
+    R.pts_to r2.state p3 r2.tl_state `star`
+    A.pts_to r2.thread_locks p4 r2.tl_thread_locks `star`
+    M.core_inv r2.tl_state `star`
+    M.frozen_logs r2.tl_state r2.tl_frozen_logs
+  ))
+
+let handle_pts_to_body
+  (r2: state_t)
+: Tot vprop
+= handle_pts_to_body0 r2
+
+[@@__reduce__]
+let state_ptr_inv_not_null_body
+  (state: R.ref state_t)
+  (st: state_t)
+: Tot vprop
+= exists_ (fun p1 ->
+    R.pts_to state p1 st `star`
+    handle_pts_to_body st
+  )
+
+[@@__reduce__]
+let state_ptr_inv_not_null
+  (state: R.ref state_t)
+: Tot vprop
+= exists_ (fun st ->
+    state_ptr_inv_not_null_body state st
+  )
 
 let state_ptr_inv_if
-  (state: R.ref M.top_level_state)
+  (state: R.ref state_t)
   (p: perm)
 : Tot vprop
 = if R.is_null state
@@ -27,7 +85,7 @@ let state_ptr_inv_if
 
 [@@__reduce__]
 let state_ptr_inv0
-  (state_ptr: R.ref (R.ref M.top_level_state))
+  (state_ptr: R.ref (R.ref state_t))
 : Tot vprop
 = exists_ (fun p -> exists_ (fun state ->
     R.pts_to state_ptr (half_perm p) state `star`
@@ -35,19 +93,19 @@ let state_ptr_inv0
   ))
 
 let state_ptr_inv
-  (state_ptr: R.ref (R.ref M.top_level_state))
+  (state_ptr: R.ref (R.ref state_t))
 : Tot vprop
 = state_ptr_inv0 state_ptr
 
 let state_ptr_lock_prop
-  (state: R.ref M.top_level_state)
+  (state: R.ref state_t)
   (p: perm)
 : Tot prop
 = R.is_null state == true ==> p == full_perm
 
 [@@__reduce__]
 let state_ptr_lock0
-  (state_ptr: R.ref (R.ref M.top_level_state))
+  (state_ptr: R.ref (R.ref state_t))
 : Tot vprop
 = exists_ (fun p -> exists_ (fun state ->
     R.pts_to state_ptr (half_perm p) state `star`
@@ -55,19 +113,19 @@ let state_ptr_lock0
   ))
 
 let state_ptr_lock
-  (state_ptr: R.ref (R.ref M.top_level_state))
+  (state_ptr: R.ref (R.ref state_t))
 : Tot vprop
 = state_ptr_lock0 state_ptr
 
 noeq
 type handle_t = {
-  state_ptr: R.ref (R.ref M.top_level_state);
+  state_ptr: R.ref (R.ref state_t);
   _inv: inv (state_ptr_inv state_ptr);
   _lock: Lock.lock (state_ptr_lock state_ptr);
 }
 
 let create_handle () : STT handle_t emp (fun _ -> emp) =
-  let state_ptr : R.ref (R.ref M.top_level_state) = R.alloc R.null in
+  let state_ptr : R.ref (R.ref state_t) = R.alloc R.null in
   R.share state_ptr;
   (* invariant *)
   rewrite (state_ptr_inv_null full_perm) (state_ptr_inv_if R.null full_perm);
@@ -94,59 +152,120 @@ let handle = create_handle ()
 assume val handle: handle_t
 
 [@@__reduce__]
+let handle_pts_to_aux0
+  (r2: state_t)
+: Tot vprop
+= exists_ (fun p1 -> exists_ (fun r1 ->
+    R.pts_to handle.state_ptr p1 r1 `star`
+    state_ptr_inv_not_null_body r1 r2
+  ))
+
+let handle_pts_to_aux
+  (r2: state_t)
+: Tot vprop
+= handle_pts_to_aux0 r2
+
+[@@__reduce__]
 let handle_pts_to0
   (ts: M.top_level_state)
 : Tot vprop
-= M.core_inv ts `star`
-  exists_ (fun p -> exists_ (fun r -> exists_ (fun p0 ->
-    R.pts_to handle.state_ptr p r `star`
-    R.pts_to r p0 ts
-  )))
+= exists_ (fun r2 ->
+    handle_pts_to_aux r2 `star`
+    pure (ts == Ghost.reveal r2.tl_state)
+  )
 
 let handle_pts_to
   (ts: M.top_level_state)
 : Tot vprop
 = handle_pts_to0 ts
 
-let handle_pts_to_core_inv_intro
-  ts
-= rewrite (handle_pts_to ts) (handle_pts_to0 ts);
+let gather_body
+  (#opened: _)
+  (r2: state_t)
+: STGhostT unit opened
+    (handle_pts_to_body r2 `star` handle_pts_to_body r2)
+    (fun _ -> handle_pts_to_body r2)
+= rewrite (handle_pts_to_body r2) (handle_pts_to_body0 r2);
   let _ = gen_elim () in
-  M.core_inv_share ts;
+  let ps = vpattern_replace (fun ps -> R.pts_to r2.state ps _) in
+  let pa = vpattern_replace (fun pa -> A.pts_to r2.thread_locks pa _) in
+  rewrite (handle_pts_to_body r2) (handle_pts_to_body0 r2);
+  let _ = gen_elim () in
+  A.gather r2.thread_locks pa _;
+  R.gather ps r2.state;
+  M.core_inv_gather _;
+  M.frozen_logs_gather _ _;
+  rewrite (handle_pts_to_body0 r2) (handle_pts_to_body r2)
+
+let gather_aux
+  (#opened: _)
+  (ts1: state_t)
+  (ts2: state_t)
+: STGhost unit opened
+    (handle_pts_to_aux ts1 `star` handle_pts_to_aux ts2)
+    (fun _ -> handle_pts_to_aux ts1)
+    True
+    (fun _ -> ts1 == ts2)
+= rewrite (handle_pts_to_aux ts1) (handle_pts_to_aux0 ts1);
+  let _ = gen_elim () in
+  let r1 = vpattern_replace (fun r1 -> R.pts_to handle.state_ptr _ r1 `star` R.pts_to r1 _ _) in
+  rewrite (handle_pts_to_aux ts2) (handle_pts_to_aux0 ts2);
+  let _ = gen_elim () in
+  let r2 = vpattern_replace (fun r2 -> R.pts_to handle.state_ptr _ r1 `star` R.pts_to handle.state_ptr _ r2 `star` R.pts_to r2 _ _) in
+  R.gather _ #r1 handle.state_ptr;
+  vpattern_rewrite #_ #_ #r2 (fun r2 -> R.pts_to r2 _ _) r1;
+  R.gather _ #ts1 r1;
+  rewrite (handle_pts_to_body ts2) (handle_pts_to_body ts1);
+  gather_body ts1;
+  rewrite (handle_pts_to_aux0 ts1) (handle_pts_to_aux ts1)
+  
+let gather ts ts' =
+  rewrite (handle_pts_to ts) (handle_pts_to0 ts);
+  let _ = gen_elim () in
+  let ts1 = vpattern_replace handle_pts_to_aux in
+  rewrite (handle_pts_to ts') (handle_pts_to0 ts');
+  let _ = gen_elim () in
+  gather_aux ts1 _;
   rewrite (handle_pts_to0 ts) (handle_pts_to ts)
 
-let handle_pts_to_core_inv_elim
-  ts
-= rewrite (handle_pts_to ts) (handle_pts_to0 ts);
+let share_body
+  (#opened: _)
+  (r2: state_t)
+: STGhostT unit opened
+    (handle_pts_to_body r2)
+    (fun _ -> handle_pts_to_body r2 `star` handle_pts_to_body r2)
+= rewrite (handle_pts_to_body r2) (handle_pts_to_body0 r2);
   let _ = gen_elim () in
-  M.core_inv_gather ts;
-  rewrite (handle_pts_to0 ts) (handle_pts_to ts)
+  let pa = vpattern_replace (fun pa -> A.pts_to r2.thread_locks pa _) in
+  A.share r2.thread_locks pa (half_perm pa) (half_perm pa);
+  R.share r2.state;
+  M.core_inv_share _;
+  M.frozen_logs_share _ _;
+  rewrite (handle_pts_to_body0 r2) (handle_pts_to_body r2);
+  noop ();
+  rewrite (handle_pts_to_body0 r2) (handle_pts_to_body r2)
 
-let gather ts1 ts2 =
-  rewrite (handle_pts_to ts1) (handle_pts_to0 ts1);
+let share_aux
+  (#opened: _)
+  (r2: state_t)
+: STGhostT unit opened
+    (handle_pts_to_aux r2)
+    (fun _ -> handle_pts_to_aux r2 `star` handle_pts_to_aux r2)
+= rewrite (handle_pts_to_aux r2) (handle_pts_to_aux0 r2);
   let _ = gen_elim () in
-  let pt1 = vpattern_replace (fun pt1 -> R.pts_to handle.state_ptr pt1 _) in
-  let p1 = vpattern_replace (fun p1 -> R.pts_to #M.top_level_state _ p1 _) in
-  rewrite (handle_pts_to ts2) (handle_pts_to0 ts2);
-  let _ = gen_elim () in
-  let p2 = vpattern_replace (fun p2 -> R.pts_to #M.top_level_state _ p1 _ `star` R.pts_to #M.top_level_state _ p2 _) in
-  R.gather pt1 handle.state_ptr;
-  let r = vpattern_replace (R.pts_to handle.state_ptr _) in 
-  vpattern_rewrite (fun (r: R.ref M.top_level_state) -> R.pts_to r p1 _) r;
-  vpattern_rewrite (fun (r: R.ref M.top_level_state) -> R.pts_to r p2 _) r;
-  R.gather p1 r;
-  rewrite (M.core_inv ts2) (M.core_inv ts1);
-  M.core_inv_gather ts1;
-  rewrite (handle_pts_to0 ts1) (handle_pts_to ts1)
+  let r1 = vpattern_replace (fun r1 -> R.pts_to handle.state_ptr _ r1 `star` R.pts_to r1 _ _) in
+  R.share handle.state_ptr;
+  R.share r1;
+  share_body r2;
+  rewrite (handle_pts_to_aux0 r2) (handle_pts_to_aux r2);
+  noop ();
+  rewrite (handle_pts_to_aux0 r2) (handle_pts_to_aux r2)
 
 let share
   ts
 = rewrite (handle_pts_to ts) (handle_pts_to0 ts);
   let _ = gen_elim () in
-  let r : R.ref M.top_level_state = vpattern_replace (fun r -> R.pts_to handle.state_ptr _ r `star` R.pts_to r _ ts) in
-  R.share handle.state_ptr;
-  R.share r;
-  M.core_inv_share ts;
+  share_aux _;
   rewrite (handle_pts_to0 ts) (handle_pts_to ts);
   noop ();
   rewrite (handle_pts_to0 ts) (handle_pts_to ts)
@@ -162,57 +281,6 @@ let with_invariant_g (#a:Type)
                                          (fun x -> p `star` fp' x))
   : STGhostT a opened_invariants fp fp'
 = with_invariant_g i f
-
-let gen_handle_pts_to_not_null
-  (#opened: _)
-  (#p: _)
-  (#state: _)
-  ()
-: STGhost (Ghost.erased M.top_level_state) opened
-    (R.pts_to handle.state_ptr p state)
-    (fun ts -> exists_ (fun p' -> R.pts_to handle.state_ptr (half_perm p') state) `star` handle_pts_to ts)
-    ((not (mem_inv opened handle._inv)) /\
-      (not (R.is_null state))
-    )
-    (fun _ -> True)
-= noop (); // for pure
-  with_invariant_g
-    #(Ghost.erased M.top_level_state)
-    #(R.pts_to handle.state_ptr p state `star` pure (R.is_null state == false))
-    #(fun ts -> (exists_ (fun p' -> R.pts_to handle.state_ptr (half_perm p') state) `star` handle_pts_to ts))
-    #opened
-    #(state_ptr_inv handle.state_ptr)
-    handle._inv
-    (fun _ ->
-      rewrite
-        (state_ptr_inv handle.state_ptr)
-        (state_ptr_inv0 handle.state_ptr);
-      let _ = gen_elim () in
-      R.gather p handle.state_ptr;
-      vpattern_rewrite (R.pts_to handle.state_ptr _) state;
-      rewrite
-        (state_ptr_inv_if _ _)
-        (state_ptr_inv_not_null state);
-      let _ = gen_elim () in
-      let ts = vpattern_replace_erased (fun ts -> R.pts_to state _ ts `star` M.core_inv ts) in
-      R.share state;
-      M.core_inv_share ts;
-      R.share handle.state_ptr;
-      (* handle_pts_to *)
-      rewrite (handle_pts_to0 ts) (handle_pts_to ts);
-      let p' = vpattern_replace (fun p' -> R.pts_to handle.state_ptr p' _) in
-      R.share handle.state_ptr;
-      (* invariant *)
-      rewrite
-        (state_ptr_inv_not_null state)
-        (state_ptr_inv_if state p');
-      rewrite
-        (state_ptr_inv0 handle.state_ptr)
-        (state_ptr_inv handle.state_ptr);
-      (* postcond *)
-      noop ();
-      ts
-    )
 
 assume
 val atomic_read_ref
@@ -241,7 +309,7 @@ val atomic_write_ref
 let handle_is_null_post (b: bool) : vprop =
   if b
   then emp
-  else exists_ handle_pts_to
+  else exists_ handle_pts_to_aux
 
 inline_for_extraction
 let with_invariant (#a:Type)
@@ -296,8 +364,9 @@ let handle_is_null
           (state_ptr_inv_not_null state);
         let _ = gen_elim () in
         R.share handle.state_ptr;
+        let r2 = vpattern_replace_erased (fun r2 -> R.pts_to state _ r2 `star` handle_pts_to_body r2) in
+        share_body _;
         R.share state;
-        M.core_inv_share _;
         (* invariant *)
         rewrite
           (state_ptr_inv_not_null state)
@@ -306,16 +375,85 @@ let handle_is_null
           (state_ptr_inv0 handle.state_ptr)
           (state_ptr_inv handle.state_ptr);
         (* handle_pts_to *)
-        let ts = vpattern_replace_erased (fun ts -> R.pts_to state _ ts `star` M.core_inv ts) in
         rewrite
-          (handle_pts_to0 ts)
-          (handle_pts_to ts);
+          (handle_pts_to_aux0 r2)
+          (handle_pts_to_aux0 r2);
         rewrite 
-          (exists_ handle_pts_to)
+          (exists_ handle_pts_to_aux)
           (handle_is_null_post false);
         return false
       end
     )
+
+let seq_lemma_index_upd
+  (#a:Type)
+  (s:Seq.seq a)
+  (n:nat{n < Seq.length s})
+  (v:a)
+: Lemma
+  (requires True)
+  (ensures (forall i . Seq.index (Seq.upd s n v) i == (if i = n then v else Seq.index s i)))
+= ()
+
+// TODO: replace this function with a Steel.ST.Loops.while_loop
+let rec init_thread_locks_loop
+  (tl_state: Ghost.erased M.top_level_state)
+  (tl_logs: Ghost.erased M.tid_log_map)
+  (tl: A.array (thread_lock_t tl_state))
+  (a0: Ghost.erased (Seq.seq (thread_lock_t tl_state)))
+  (tid: U16.t)
+: ST unit
+    (M.all_logs tl_state tl_logs `star` A.pts_to tl full_perm a0)
+    (fun _ ->
+      exists_ (fun l' -> M.frozen_logs tl_state l') `star`
+      exists_ (fun a ->
+      A.pts_to tl full_perm a `star`
+      pure (thread_state_prop a /\ Seq.length a == U32.v AT.n_threads)
+    ))
+    (A.length tl == U32.v AT.n_threads /\
+      Seq.length (Ghost.reveal a0) == U32.v AT.n_threads /\
+      U16.v tid <= U32.v AT.n_threads /\
+      (forall (i: nat) . i < U16.v tid ==> U16.v (Ghost.reveal (dfst (Seq.index (Ghost.reveal a0) i))) == i) /\
+      (forall (i: AT.tid) . U16.v i >= U16.v tid ==> Some? (Map.sel tl_logs i))
+    )
+    (fun _ -> True)
+= let tid32 = FStar.Int.Cast.uint16_to_uint32 tid in
+  if tid32 = AT.n_threads
+  then begin
+    M.freeze_all_logs _ _;
+    return ()
+  end
+  else begin
+    M.all_logs_log_of_tid _ _ tid ();
+    let l = Lock.new_lock (thread_lock_vprop tl_state tid) in
+    let t : thread_lock_t tl_state = (| Ghost.hide tid, l |) in
+    A.write tl tid32 t;
+    Seq.lemma_len_upd (U32.v tid32) t a0;
+    seq_lemma_index_upd a0 (U32.v tid32) t;
+    init_thread_locks_loop tl_state _ tl _ (tid `U16.add` 1us)
+  end
+
+let init_thread_locks
+  (tl_state: Ghost.erased M.top_level_state)
+  (tl_logs: Ghost.erased M.tid_log_map)
+: ST (A.array (thread_lock_t tl_state))
+    (M.all_logs tl_state tl_logs)
+    (fun tl ->
+      exists_ (fun l' -> M.frozen_logs tl_state l') `star`
+      exists_ (fun a ->
+        A.pts_to tl full_perm a `star`
+        pure (thread_state_prop a /\ Seq.length a == U32.v AT.n_threads)
+    ))
+    (forall (i: AT.tid) . Some? (Map.sel tl_logs i))
+    (fun _ -> True)
+= M.all_logs_log_of_tid _ _ 0us ();
+  let l0 = Lock.new_lock (thread_lock_vprop tl_state 0us) in
+  let tl0: thread_lock_t tl_state = (| Ghost.hide 0us, l0 |) in
+  let tl = A.alloc tl0 AT.n_threads in
+  Seq.lemma_create_len (U32.v AT.n_threads) tl0;
+  Seq.lemma_index_create (U32.v AT.n_threads) tl0 0;
+  init_thread_locks_loop _ _ tl _ 1us;
+  return tl
 
 #push-options "--z3rlimit 32"
 #restart-solver
@@ -327,15 +465,35 @@ let init ()
   let state = R.read handle.state_ptr in
   if R.is_null state
   then begin
-    let state' = M.init () in
+    let r2_state = M.init () in
     let ts = elim_exists () in
+    let tl = init_thread_locks ts _ in
+    let _ = gen_elim () in
+    let tl_f = vpattern_replace_erased (M.frozen_logs ts) in
+    let tl_a = vpattern_replace_erased (A.pts_to tl _) in
+    [@@inline_let]
+    let r2 = ({
+      state = r2_state;
+      tl_state = ts;
+      thread_locks = tl;
+      tl_thread_locks = tl_a;
+      tl_frozen_logs = tl_f;
+      tl_prf = ();
+    })
+    in
+    let state' = R.alloc r2 in
     R.pts_to_not_null state';
+    rewrite (R.pts_to r2_state full_perm _) (R.pts_to r2.state full_perm r2.tl_state);
+    rewrite (A.pts_to _ _ _) (A.pts_to r2.thread_locks full_perm r2.tl_thread_locks);
+    rewrite (M.frozen_logs _ _) (M.frozen_logs r2.tl_state r2.tl_frozen_logs);
     rewrite (R.pts_to handle.state_ptr _ _) (R.pts_to handle.state_ptr (half_perm full_perm) state);
-    M.core_inv_share ts;
+    vpattern_rewrite M.core_inv (Ghost.reveal r2.tl_state);
+    rewrite (handle_pts_to_body0 r2) (handle_pts_to_body r2);
+    share_body _;
     R.share state';
     with_invariant
       #unit
-      #(R.pts_to handle.state_ptr (half_perm full_perm) state `star` R.pts_to state' (half_perm full_perm) ts `star` M.core_inv ts)
+      #(R.pts_to handle.state_ptr (half_perm full_perm) state `star` R.pts_to state' (half_perm full_perm) r2 `star` handle_pts_to_body r2)
       #(fun _ -> R.pts_to handle.state_ptr (half_perm full_perm) state')
       #_
       #(state_ptr_inv handle.state_ptr)
@@ -352,45 +510,84 @@ let init ()
         vpattern_rewrite (fun p -> R.pts_to handle.state_ptr p _) full_perm;
         atomic_write_ref handle.state_ptr state';
         R.share handle.state_ptr;
-        noop ();
         rewrite
           (state_ptr_inv_not_null state')
           (state_ptr_inv_if state' full_perm);
         rewrite
           (state_ptr_inv0 handle.state_ptr)
-          (state_ptr_inv handle.state_ptr)
+          (state_ptr_inv handle.state_ptr);
+        noop ()
       );
     R.share handle.state_ptr;
     rewrite (state_ptr_lock0 handle.state_ptr) (state_ptr_lock handle.state_ptr);
     Lock.release handle._lock;
+    rewrite (handle_pts_to_aux0 r2) (handle_pts_to_aux r2);
     rewrite (handle_pts_to0 ts) (handle_pts_to ts);
-    rewrite (init_post_true ts) (init_post true ts);
     return true
   end else begin
-    let ts = gen_handle_pts_to_not_null () in
-    let _ = gen_elim () in
+    R.share handle.state_ptr;
     rewrite (state_ptr_lock0 handle.state_ptr) (state_ptr_lock handle.state_ptr);
     Lock.release handle._lock;
-    rewrite emp (init_post false ts);
+    let p = vpattern_replace (fun p -> R.pts_to handle.state_ptr p _) in
+    rewrite (R.pts_to handle.state_ptr _ _) (R.pts_to handle.state_ptr p state);
+    with_invariant_g
+      #unit
+      #(R.pts_to handle.state_ptr p state)
+      #(fun _ -> exists_ (fun ts -> handle_pts_to ts))
+      #_
+      #(state_ptr_inv handle.state_ptr)
+      handle._inv
+      (fun _ ->
+        rewrite (state_ptr_inv _) (state_ptr_inv0 handle.state_ptr);
+        let _ = gen_elim () in
+        R.gather _ #state handle.state_ptr;
+        rewrite (state_ptr_inv_if _ _) (state_ptr_inv_not_null state);
+        let _ = gen_elim () in
+        R.share state;
+        share_body _;
+        let p' = vpattern_replace (fun p -> R.pts_to handle.state_ptr p _) in
+        R.share handle.state_ptr;
+        rewrite (state_ptr_inv_not_null state) (state_ptr_inv_if state p');
+        rewrite (state_ptr_inv0 handle.state_ptr) (state_ptr_inv handle.state_ptr);
+        let r2 = vpattern_replace (fun r2 -> R.pts_to state _ r2 `star` handle_pts_to_body r2) in
+        let ts = Ghost.reveal r2.tl_state in
+        rewrite (handle_pts_to_aux0 r2) (handle_pts_to_aux r2);
+        rewrite (handle_pts_to0 ts) (handle_pts_to ts);
+        noop ()
+      );
     return false
   end
 
 #pop-options
 
-assume val acquire_thread_lock
-  (t: Ghost.erased M.top_level_state)
+inline_for_extraction
+let acquire_thread_lock
+  (t: state_t)
   (tid: AT.tid)
 : STT (Ghost.erased AEH.log)
-    (handle_pts_to t)
-    (fun entries -> handle_pts_to t `star` M.log_of_tid t tid entries)
+    (handle_pts_to_body t)
+    (fun entries -> handle_pts_to_body t `star` M.log_of_tid t.tl_state tid entries)
+= rewrite (handle_pts_to_body t) (handle_pts_to_body0 t);
+  let _ = gen_elim () in
+  let l = A.read t.thread_locks (FStar.Int.Cast.uint16_to_uint32 tid) in
+  Lock.acquire (dsnd l <: Lock.lock (thread_lock_vprop t.tl_state tid));
+  let entries : Ghost.erased AEH.log = elim_exists () in
+  rewrite (handle_pts_to_body0 t) (handle_pts_to_body t);
+  return entries
 
-assume val release_thread_lock
-  (t: Ghost.erased (M.top_level_state))
+inline_for_extraction
+let release_thread_lock
+  (t: state_t)
   (tid: AT.tid)
   (entries: Ghost.erased AEH.log)
 : STT unit
-    (handle_pts_to t `star` M.log_of_tid t tid entries)
-    (fun _ -> handle_pts_to t)
+    (handle_pts_to_body t `star` M.log_of_tid t.tl_state tid entries)
+    (fun _ -> handle_pts_to_body t)
+= rewrite (handle_pts_to_body t) (handle_pts_to_body0 t);
+  let _ = gen_elim () in
+  let l = A.read t.thread_locks (FStar.Int.Cast.uint16_to_uint32 tid) in
+  Lock.release (dsnd l <: Lock.lock (thread_lock_vprop t.tl_state tid));
+  rewrite (handle_pts_to_body0 t) (handle_pts_to_body t)
 
 #push-options "--z3rlimit 32 --query_stats --ifuel 6"
 #restart-solver
@@ -431,7 +628,7 @@ let m_verify_post_failure_eq
        exists_ (fun entries' -> M.log_of_tid t tid entries')))
 
 let verify_log_some
-               (t: Ghost.erased M.top_level_state)
+               (t0: Ghost.erased state_t)
                (tid:U16.t)
                (#log_perm:perm)
                (#log_bytes:Ghost.erased AT.bytes)
@@ -441,35 +638,42 @@ let verify_log_some
                (#out_bytes:Ghost.erased AT.bytes)
                (output: EXT.extern_ptr U8.t)
   : ST (verify_result len)
-    (handle_pts_to t `star` verify_pre log_perm log_bytes input out_bytes output)
+    (handle_pts_to_aux t0 `star` verify_pre log_perm log_bytes input out_bytes output)
     (fun res -> verify_post tid log_perm log_bytes len input out_len out_bytes output res)
     (check_verify_input tid len input out_len output)
     (fun _ -> True)
-= let entries = acquire_thread_lock t tid in
-  rewrite (handle_pts_to t) (handle_pts_to0 t);
+= rewrite (handle_pts_to_aux t0) (handle_pts_to_aux0 t0);
   let _ = gen_elim () in
-  let state = R.read handle.state_ptr in
-  vpattern_rewrite (R.pts_to handle.state_ptr _) state;
-  vpattern_rewrite (fun (state: R.ref M.top_level_state) -> R.pts_to state _ t) state;
+  let r1 = R.read handle.state_ptr in
+  vpattern_rewrite (fun r1 -> R.pts_to handle.state_ptr _ r1 `star` R.pts_to r1 _ _) r1;
+  let r2 = R.read r1 in
+  vpattern_rewrite (fun r2 -> R.pts_to r1 _ r2 `star` handle_pts_to_body r2) r2;
+  let entries = acquire_thread_lock _ tid in
+  rewrite (handle_pts_to_body r2) (handle_pts_to_body0 r2);
+  let _ = gen_elim () in
   let input' = EXT.take input len in
   let output' = EXT.take output out_len in
   vpattern_rewrite (fun a -> A.pts_to a log_perm log_bytes) input';
   vpattern_rewrite (fun a -> A.pts_to a full_perm out_bytes) output';
-  let v = M.verify_log state tid len input' out_len output' in
+  let v = M.verify_log _ tid len input' out_len output' in
   let res = Some v in
-  match v returns STT (verify_result len) (R.pts_to handle.state_ptr _ _ `star` R.pts_to state _ _ `star`  M.verify_post t tid entries log_perm log_bytes len input' out_len out_bytes output' v) (fun res -> verify_post tid log_perm log_bytes len input out_len out_bytes output res) with
+  let t = r2.tl_state in
+  match v returns STT (verify_result len) (R.pts_to handle.state_ptr _ r1 `star` R.pts_to r1 _ r2 `star` R.pts_to r2.state _ _ `star` A.pts_to r2.thread_locks _ _ `star` M.frozen_logs _ _ `star` M.verify_post _ tid entries log_perm log_bytes len input' out_len out_bytes output' v) (fun res -> verify_post tid log_perm log_bytes len input out_len out_bytes output res) with
   | Some (V.Verify_success read wrote) ->
     rewrite
-      (M.verify_post t tid entries log_perm log_bytes len input' out_len out_bytes output' _)
-      (M.core_inv t `star`
+      (M.verify_post _ tid entries log_perm log_bytes len input' out_len out_bytes output' _)
+      (M.core_inv r2.tl_state `star`
         A.pts_to (EXT.gtake input) log_perm log_bytes `star`
         exists_ (M.verify_post_success_pred t tid entries log_bytes out_len out_bytes output' read wrote)
       );
     let _ = gen_elim () in
-    rewrite (handle_pts_to0 t) (handle_pts_to t);
+    rewrite (handle_pts_to_body0 r2) (handle_pts_to_body r2);
     let entries' = vpattern_erased (fun entries' -> M.log_of_tid t tid (_ `Seq.append` entries')) in
+    vpattern_rewrite (fun t -> M.log_of_tid t _ _) r2.tl_state;
+    release_thread_lock _ tid _;
+    rewrite (handle_pts_to_aux0 r2) (handle_pts_to_aux r2);
+    rewrite (handle_pts_to0 t) (handle_pts_to t);
     let out_bytes' = vpattern_replace_erased (A.pts_to output' _) in
-    release_thread_lock t tid _;
     vpattern_rewrite #_ #_ #output' (fun output -> A.pts_to output _ _) (EXT.gtake output);
     assert_ (verify_post_some_m_success_body tid log_perm log_bytes len input out_len out_bytes output v () t entries read wrote entries' out_bytes');
     rewrite
@@ -480,10 +684,13 @@ let verify_log_some
       (verify_post tid log_perm log_bytes len input out_len out_bytes output res);
     return res
   | v ->
-    m_verify_post_failure_eq t tid entries log_perm log_bytes len input' out_len out_bytes output' v;
+    m_verify_post_failure_eq r2.tl_state tid entries log_perm log_bytes len input' out_len out_bytes output' v;
     let _ = gen_elim () in
+    rewrite (handle_pts_to_body0 r2) (handle_pts_to_body r2);
+    vpattern_rewrite (fun t -> M.log_of_tid t _ _) r2.tl_state;
+    release_thread_lock _ tid _;
+    rewrite (handle_pts_to_aux0 r2) (handle_pts_to_aux r2);
     rewrite (handle_pts_to0 t) (handle_pts_to t);
-    release_thread_lock t tid _;
     vpattern_rewrite #_ #_ #output' (fun output -> A.pts_to output _ _) (EXT.gtake output);
     rewrite
       (verify_post_some_m_failure output)
@@ -517,7 +724,7 @@ let verify_log
   end else 
   begin
     noop ();
-    rewrite (handle_is_null_post _) (exists_ handle_pts_to);
+    rewrite (handle_is_null_post _) (exists_ handle_pts_to_aux);
     let ts = elim_exists () in
     verify_log_some ts tid len input out_len output
   end
@@ -534,14 +741,21 @@ let max_certified_epoch
   end else 
   begin
     noop ();
-    rewrite (handle_is_null_post _) (exists_ handle_pts_to);
-    let t = elim_exists () in
-    rewrite (handle_pts_to t) (handle_pts_to0 t);
+    rewrite (handle_is_null_post _) (exists_ handle_pts_to_aux);
+    let t0 = elim_exists () in
+    rewrite (handle_pts_to_aux t0) (handle_pts_to_aux0 t0);
     let _ = gen_elim () in
-    let state = R.read handle.state_ptr in
-    vpattern_rewrite (R.pts_to handle.state_ptr _) state;
-    vpattern_rewrite (fun (state: R.ref M.top_level_state) -> R.pts_to state _ t) state;
-    let r = M.max_certified_epoch state in
+    let r1 = R.read handle.state_ptr in
+    vpattern_rewrite (fun r1 -> R.pts_to handle.state_ptr _ r1 `star` R.pts_to r1 _ _) r1;
+    let r2 = R.read r1 in
+    vpattern_rewrite (fun r2 -> R.pts_to r1 _ r2 `star` handle_pts_to_body r2) r2;
+    rewrite (handle_pts_to_body r2) (handle_pts_to_body0 r2);
+    let _ = gen_elim () in
+    let t = r2.tl_state in
+    let r = M.max_certified_epoch r2.state in
+    vpattern_rewrite (fun t -> M.read_max_post t _) t;
+    rewrite (handle_pts_to_body0 r2) (handle_pts_to_body r2);
+    rewrite (handle_pts_to_aux0 r2) (handle_pts_to_aux r2);
     rewrite (handle_pts_to0 t) (handle_pts_to t);
     let res = Some r in
     rewrite (max_certified_epoch_post_some r) (max_certified_epoch_post res);
